Original_Dinitz_Refine.thy
@@ -1057,131 +1057,19 @@ end
 \<comment> \<open>Building a dual layering\<close>
 \<comment> \<open>Extended BFS\<close>
 
-
-
-
-
-
-
-
-
-
-
-
-
-
-
-
-
-
-
-
-
-
-
-
-
-
 subsection \<open>Dinitz phase refinement\<close>
 
-
-
-
-
-(* TODO *)
-end
-
-
-
+subsubsection \<open>Abstract version with assertions\<close>
 context NFlow
 begin
-
-section \<open>Experiment\<close>
-definition test1 :: "_ flow nres" where
-  "test1 \<equiv> do {
-    (f', _, _) \<leftarrow> WHILE\<^sub>T
-      (\<lambda>(_, _, brk). \<not> brk)
-      (\<lambda>(f', stl, _). do {
-            stl \<leftarrow> Graph.subtract_path_algo stl [(0, 0)];
-            RETURN (f', stl, False)
-          })
-      (f, c, False);
-    RETURN f'}"
-definition test2 :: "_ flow nres" where
-  "test2 \<equiv> do {
-    (f', _, _) \<leftarrow> WHILE\<^sub>T
-      (\<lambda>(_, _, brk). \<not> brk)
-      (\<lambda>(f', stl, _). do {
-            stl \<leftarrow> return (Graph.subtract_path stl [(0, 0)]);
-            RETURN (f', stl, False)
-          })
-      (f, c, False);
-    RETURN f'}"
-
-thm refine_dref_pattern
-(* TODO find out which rule leads to the spec term, which in turn means dref_type cannot infer relation type *)
-lemma "test1 \<le> \<Down> Id test2"
-  unfolding test1_def test2_def
-  apply refine_rcg
-         apply refine_dref_type
-      apply clarsimp_all
-  oops
-\<comment> \<open>Experiment\<close>
-
-
-
-
-
-(* TODO *)
-(*declare fun_relI[refine del]*)
-lemma RELATESI_workaround[refine_dref_pattern]:
-  "RELATES R \<Longrightarrow> S \<le> (spec x. (x, y) \<in> R) \<Longrightarrow> S \<le> (spec x. (x, y) \<in> R)" .
-
-
-thm build_st_layering_correct
-  Dual_Layer_Graph.greedyPathFinding_correct
-  subtract_path_algo_correct
-  Graph.inner_path_vertices_algo_correct
-  Finite_Bounded_Graph.cleaning_algo_correct
-
-(* TODO cleanup assertions *)
-
-(*
-definition dinitz_phase_assert_invar :: "(_ flow \<times> _ graph \<times> bool) \<Rightarrow> bool" where
-  "dinitz_phase_assert_invar \<equiv> \<lambda>(f', stl, brk).
+text \<open>Now that we have refined all the sub-algorithms we need, we shall start refining the entire
+      Dinitz algorithm. The first step is introducing and proving a few assertions we needed to
+      assume for the previous correctness proof.\<close>
+(* TODO move the restructured version to Dinitz_Algo and merely prove assertions here *)
+definition dinitzPhaseAssertInvar :: "(_ flow \<times> _ graph \<times> bool \<times> bool) \<Rightarrow> bool" where
+  "dinitzPhaseAssertInvar \<equiv> \<lambda>(f', stl, brk, changed).
     NFlow c s t f'
-    \<and> Bounded_ST_Shortest_Path_Union stl (cf_of f') s t (cf.min_dist s t)
-    \<and> (Graph.connected (cf_of f') s t \<longrightarrow> cf.min_dist s t \<le> Graph.min_dist (cf_of f') s t)
-    \<and> (brk \<longrightarrow> \<not> Graph.connected stl s t)"
-
-definition dinitz_phase_assert :: "_ flow nres" where
-  "dinitz_phase_assert \<equiv> do {
-    stl \<leftarrow> (spec c'. ST_Shortest_Path_Union c' cf s t);
-    (f', _, _) \<leftarrow> WHILE\<^sub>T\<^bsup>dinitz_phase_assert_invar\<^esup>
-      (\<lambda>(_, _, brk). \<not> brk)
-      (\<lambda>(f', stl, _). do {
-        p' \<leftarrow> select p. Graph.isPath stl s p t;
-        case p' of
-          None \<Rightarrow> RETURN (f', stl, True)
-        | Some p \<Rightarrow> do {
-            assert (Graph.isPath stl s p t);
-            assert (ST_Shortest_Path_Union stl (cf_of f') s t);
-            Q_ls \<leftarrow> return (tl (butlast (Graph.pathVertices s p)));
-            assert (set Q_ls = set (Graph.pathVertices s p) - {s, t});
-            stl' \<leftarrow> return (Graph.subtract_path stl p);
-            assert (Contained_Graph stl' stl \<and> Graph.E stl \<subseteq> Graph.E stl' \<union> set p);
-            stl' \<leftarrow> return (cleaning s t stl');
-            let f' = NFlow.augment c f' (NPreflow.augmentingFlow c f' p);
-            RETURN (f', stl', False)
-          }})
-      (f, stl, False);
-    RETURN f'}"
-*)
-
-definition dinitz_phase_assert_invar :: "(_ flow \<times> _ graph \<times> bool \<times> bool) \<Rightarrow> bool" where
-  "dinitz_phase_assert_invar \<equiv> \<lambda>(f', stl, brk, changed).
-    NFlow c s t f'
-    \<and> Bounded_ST_Shortest_Path_Union stl (cf_of f') s t (cf.min_dist s t)
+    \<and> Bounded_Dual_Shortest_Path_Union stl (cf_of f') s t (cf.min_dist s t)
     \<and> (Graph.connected (cf_of f') s t \<longrightarrow> cf.min_dist s t \<le> Graph.min_dist (cf_of f') s t)
     \<and> (brk \<longrightarrow> \<not> Graph.connected stl s t)
     \<and> (val \<le> Flow.val c s f')
@@ -1189,19 +1077,19 @@ definition dinitz_phase_assert_invar :: "(_ flow \<times> _ graph \<times> bool 
     \<and> (changed \<longrightarrow> cf.connected s t)" (* \<and> (changed \<and> brk \<longrightarrow> cf.connected s t)" *)
 
 (* TODO can this be simplified to just changed \<longleftrightarrow> val < val'? *)
-lemma dinitz_phase_assert_invar_alt:
-  "dinitz_phase_assert_invar = (\<lambda>(f', stl, brk, changed).
-    dinitz_phase_invar (f', stl)
+lemma dinitzPhaseAssertInvar_alt:
+  "dinitzPhaseAssertInvar = (\<lambda>(f', stl, brk, changed).
+    dinitzPhaseInvar (f', stl)
     \<and> (brk \<longrightarrow> \<not> Graph.connected stl s t)
     \<and> (val \<le> Flow.val c s f')
     \<and> (changed \<longleftrightarrow> f' \<noteq> f)
     \<and> (changed \<longrightarrow> cf.connected s t))" (* TODO does this work? *)
-  unfolding dinitz_phase_invar_def dinitz_phase_assert_invar_def by simp
+  unfolding dinitzPhaseInvar_def dinitzPhaseAssertInvar_def by simp
 
-definition dinitz_phase_assert :: "(_ flow \<times> bool) nres" where
-  "dinitz_phase_assert \<equiv> do {
-    stl \<leftarrow> (spec c'. ST_Shortest_Path_Union c' cf s t);
-    (f', _, _, changed) \<leftarrow> WHILE\<^sub>T\<^bsup>dinitz_phase_assert_invar\<^esup>
+definition dinitzPhaseAssert :: "(_ flow \<times> bool) nres" where
+  "dinitzPhaseAssert \<equiv> do {
+    stl \<leftarrow> (spec c'. Dual_Shortest_Path_Union c' cf s t);
+    (f', _, _, changed) \<leftarrow> WHILE\<^sub>T\<^bsup>dinitzPhaseAssertInvar\<^esup>
       (\<lambda>(_, _, brk, _). \<not> brk)
       (\<lambda>(f', stl, _, changed). do {
         p' \<leftarrow> select p. Graph.isPath stl s p t;
@@ -1209,7 +1097,7 @@ definition dinitz_phase_assert :: "(_ flow \<times> bool) nres" where
           None \<Rightarrow> RETURN (f', stl, True, changed)
         | Some p \<Rightarrow> do {
             assert (Graph.isPath stl s p t);
-            assert (ST_Shortest_Path_Union stl (cf_of f') s t);
+            assert (Dual_Shortest_Path_Union stl (cf_of f') s t);
             Q_ls \<leftarrow> return (tl (butlast (Graph.pathVertices s p)));
             assert (set Q_ls = set (Graph.pathVertices s p) - {s, t});
             stl' \<leftarrow> return (Graph.subtract_path stl p);
@@ -1224,44 +1112,44 @@ definition dinitz_phase_assert :: "(_ flow \<times> bool) nres" where
 (* TODO comment about val needed for changed inequality *)
 
 (* TODO use this in phase step *)
-lemma stu_if_invar_and_path:
-  assumes INVAR: "dinitz_phase_invar (f', stl)"
+lemma dual_spu_if_invar_and_path:
+  assumes INVAR: "dinitzPhaseInvar (f', stl)"
     and PATH: "Graph.isPath stl s p t"
-  shows "ST_Shortest_Path_Union stl (cf_of f') s t"
+  shows "Dual_Shortest_Path_Union stl (cf_of f') s t"
 proof -
-  from INVAR interpret f': NFlow c s t f' unfolding dinitz_phase_invar_def by blast
+  from INVAR interpret f': NFlow c s t f' unfolding dinitzPhaseInvar_def by blast
 
   have BOUND_EQ: "cf.min_dist s t = f'.cf.min_dist s t"
   proof -
-    from INVAR interpret Bounded_ST_Shortest_Path_Union stl f'.cf s t "cf.min_dist s t"
-      unfolding dinitz_phase_invar_def by simp
+    from INVAR interpret Bounded_Dual_Shortest_Path_Union stl f'.cf s t "cf.min_dist s t"
+      unfolding dinitzPhaseInvar_def by simp
     show ?thesis
     proof (intro antisym)
       from PATH INVAR show "cf.min_dist s t \<le> f'.cf.min_dist s t"
-        unfolding dinitz_phase_invar_def Graph.connected_def
+        unfolding dinitzPhaseInvar_def Graph.connected_def
         using sg_paths_are_base_paths by blast
       from PATH show "f'.cf.min_dist s t \<le> cf.min_dist s t" (* TODO fix proof *)
       using f'.cf.isShortestPath_min_dist_def path_length_bounded shortest_path_transfer (* by simp *)
       by (metis Bounded_Shortest_Path_Union.obtain_close_ST Bounded_Shortest_Path_Union_axioms emptyE g'.isEmpty_def g'.isPath_bwd_cases min_dist_transfer s_in_V_if_nonempty singleton_iff t_not_s)
     qed
   qed
-  with INVAR show "ST_Shortest_Path_Union stl (f'.cf) s t"
-    unfolding dinitz_phase_invar_def using min_st_dist_bound by fastforce
+  with INVAR show "Dual_Shortest_Path_Union stl (f'.cf) s t"
+    unfolding dinitzPhaseInvar_def using min_st_dist_bound by fastforce
 qed
 
-lemma dinitz_phase_assert_step:
+lemma dinitzPhaseAssert_step:
   fixes f' stl changed
   assumes PATH: "Graph.isPath stl s p t"
-      and INVAR: "dinitz_phase_assert_invar (f', stl, False, changed)"
+      and INVAR: "dinitzPhaseAssertInvar (f', stl, False, changed)"
   defines "aug_f' \<equiv> NFlow.augment c f' (NPreflow.augmentingFlow c f' p)"
       and "stl' \<equiv> cleaning s t (Graph.subtract_path stl p)"
-    shows "dinitz_phase_assert_invar (aug_f', stl', False, True) \<and> Graph.E stl' \<subset> Graph.E stl \<and> finite (Graph.E stl)"
+    shows "dinitzPhaseAssertInvar (aug_f', stl', False, True) \<and> Graph.E stl' \<subset> Graph.E stl \<and> finite (Graph.E stl)"
 proof -
   have "Flow.val c s f' < Flow.val c s aug_f'"
   proof -
-    from INVAR interpret f': NFlow c s t f' unfolding dinitz_phase_assert_invar_def by blast
-    from INVAR PATH interpret stu: ST_Shortest_Path_Union stl "cf_of f'" s t
-      unfolding dinitz_phase_assert_invar_alt using stu_if_invar_and_path by blast
+    from INVAR interpret f': NFlow c s t f' unfolding dinitzPhaseAssertInvar_def by blast
+    from INVAR PATH interpret stu: Dual_Shortest_Path_Union stl "cf_of f'" s t
+      unfolding dinitzPhaseAssertInvar_alt using dual_spu_if_invar_and_path by blast
 
     have "Flow f'.cf s t (f'.augmentingFlow p)"
       apply (intro f'.augFlow_resFlow)
@@ -1271,50 +1159,42 @@ proof -
       by (simp add: Graph.shortestPath_is_path Graph.shortestPath_is_simple PATH f'.augFlow_val f'.isAugmentingPath_def f'.resCap_gzero_aux stu.shortest_path_transfer)
     ultimately show ?thesis unfolding aug_f'_def using f'.augment_flow_value by simp
   qed
-  with PATH INVAR show ?thesis unfolding dinitz_phase_assert_invar_alt aug_f'_def stl'_def
+  with PATH INVAR show ?thesis unfolding dinitzPhaseAssertInvar_alt aug_f'_def stl'_def
     using dinitz_phase_step (* TODO prettify *)
     apply auto
-    apply (meson Graph.connected_def ST_Shortest_Path_Union.st_connected_iff stu_if_invar_and_path)
+    apply (meson Graph.connected_def Dual_Shortest_Path_Union.st_connected_iff dual_spu_if_invar_and_path)
     by blast+
 qed
 
-
-
-
-definition "dinitz_phase_assert_wf_rel \<equiv> inv_image
+definition "dinitzPhaseAssert_wf_rel \<equiv> inv_image
   (less_than_bool <*lex*> finite_psubset)
   (\<lambda>(_, stl, brk, _). (\<not>brk, Graph.E stl))"
 
-
-find_theorems Graph.E Graph.subtract_path
-find_theorems Graph.E Graph.subtract_graph
-thm Graph.subtract_graph_untouched_edges
-
-lemma dinitz_phase_assert_correct:
-  "dinitz_phase_assert \<le> SPEC (\<lambda>(f', changed). res_dist_increasing_flow f' \<and> changed = (f' \<noteq> f) \<and> (changed \<longrightarrow> cf.connected s t))"
-  unfolding dinitz_phase_assert_def
-  apply (refine_vcg WHILEIT_rule[where R=dinitz_phase_assert_wf_rel])
+lemma dinitzPhaseAssert_correct:
+  "dinitzPhaseAssert \<le> SPEC (\<lambda>(f', changed). res_dist_increasing_flow f' \<and> changed = (f' \<noteq> f) \<and> (changed \<longrightarrow> cf.connected s t))"
+  unfolding dinitzPhaseAssert_def
+  apply (refine_vcg WHILEIT_rule[where R=dinitzPhaseAssert_wf_rel])
                       apply (all \<open>(clarsimp; fail)?\<close>)
-            apply (simp add: dinitz_phase_assert_wf_rel_def wf_lex_prod)
-            apply (simp add: dinitz_phase_assert_invar_def NFlow_axioms min_st_dist_bound)
+            apply (simp add: dinitzPhaseAssert_wf_rel_def wf_lex_prod)
+            apply (simp add: dinitzPhaseAssertInvar_def NFlow_axioms min_st_dist_bound)
            defer defer defer
   apply (simp add: Graph.subtract_path_alt) using Graph.subtract_graph_untouched_edges apply (metis (no_types, lifting) Graph.isPath_alt Graph.path_induced_graph_edges Int_Un_eq(4) Int_absorb1 Int_commute Un_Diff_cancel2 cf.isPath.simps(1) set_eq_subset t_not_s)
-          apply (simp add: dinitz_phase_assert_step)
-          apply (simp add: dinitz_phase_assert_step dinitz_phase_assert_wf_rel_def)
-        apply (simp add: dinitz_phase_assert_invar_alt Graph.connected_def)
-       apply (simp add: dinitz_phase_assert_wf_rel_def)
-      apply (clarsimp simp: dinitz_phase_assert_invar_alt dinitz_phase_final)
-      apply (simp add: dinitz_phase_assert_invar_alt)
-  apply (clarsimp simp: dinitz_phase_assert_invar_alt)
-proof clarsimp_all oops
+          apply (simp add: dinitzPhaseAssert_step)
+          apply (simp add: dinitzPhaseAssert_step dinitzPhaseAssert_wf_rel_def)
+        apply (simp add: dinitzPhaseAssertInvar_alt Graph.connected_def)
+       apply (simp add: dinitzPhaseAssert_wf_rel_def)
+      apply (clarsimp simp: dinitzPhaseAssertInvar_alt dinitz_phase_final)
+      apply (simp add: dinitzPhaseAssertInvar_alt)
+  apply (clarsimp simp: dinitzPhaseAssertInvar_alt)
+proof clarsimp_all
   fix f' stl p changed
   interpret cf': Graph "cf_of f'" .
-  assume INVAR: "dinitz_phase_assert_invar (f', stl, False, changed)" and PATH: "Graph.isPath stl s p t"
-  then show "ST_Shortest_Path_Union stl (cf_of f') s t"
-    unfolding dinitz_phase_assert_invar_alt using stu_if_invar_and_path by blast
-  then interpret ST_Shortest_Path_Union stl "cf_of f'" s t .
+  assume INVAR: "dinitzPhaseAssertInvar (f', stl, False, changed)" and PATH: "Graph.isPath stl s p t"
+  then show "Dual_Shortest_Path_Union stl (cf_of f') s t"
+    unfolding dinitzPhaseAssertInvar_alt using dual_spu_if_invar_and_path by blast
+  then interpret Dual_Shortest_Path_Union stl "cf_of f'" s t .
 
-  from INVAR interpret f': NFlow c s t f' unfolding dinitz_phase_assert_invar_def by blast
+  from INVAR interpret f': NFlow c s t f' unfolding dinitzPhaseAssertInvar_def by blast
   interpret g': Nonnegative_Graph stl
     using f'.cf.Nonnegative_Graph_axioms sg_Nonnegative_Graph by blast
   (* TODO replace this with a simple 'have', need some way to use sublocale relations *)
@@ -1333,85 +1213,66 @@ proof clarsimp_all oops
   then show "set (tl (butlast (pathVertices s p))) = set (pathVertices s p) - {s, t}"
     by (smt (verit, ccfv_threshold) Diff_insert0 Graph.isSimplePath_fwd Graph.pathVertices_fwd PATH Un_Diff_Int Un_insert_right distinct.simps(2) distinct_append empty_set insertCI insert_Diff1 list.simps(15) paths_are_simple set_append sup_bot.right_neutral)
 qed
+end
+\<comment> \<open>Abstract version with assertions\<close>
 
-definition dinitz_phase_concrete :: "(_ flow \<times> bool) nres" where
-  "dinitz_phase_concrete \<equiv> do {
-    stl \<leftarrow> cf.build_st_layering s t;
-    (f', _, _, changed) \<leftarrow> WHILE\<^sub>T\<^bsup>dinitz_phase_assert_invar\<^esup>
+subsubsection \<open>Refining the assertion version\<close>
+context NFlow
+begin
+(* TODO prettify Q_ls *)
+definition dinitzPhaseRefine :: "(_ flow \<times> bool) nres" where
+  "dinitzPhaseRefine \<equiv> do {
+    stl \<leftarrow> cf.buildDualLayering s t;
+    (f', _, _, changed) \<leftarrow> WHILE\<^sub>T\<^bsup>dinitzPhaseAssertInvar\<^esup>
       (\<lambda>(_, _, brk, _). \<not> brk)
       (\<lambda>(f', stl, _, changed). do {
-        p' \<leftarrow> Graph.greedy_st_path_finding stl s t;
+        p' \<leftarrow> Graph.greedyPathFinding stl s t;
         case p' of
           None \<Rightarrow> RETURN (f', stl, True, changed)
         | Some p \<Rightarrow> do {
             assert (Graph.isPath stl s p t);
-            assert (ST_Shortest_Path_Union stl (cf_of f') s t);
-            Q_ls \<leftarrow> inner_path_vertices_algo p;
+            assert (Dual_Shortest_Path_Union stl (cf_of f') s t);
+            let Q_ls = innerPathVertices p;
             assert (set Q_ls = set (Graph.pathVertices s p) - {s, t});
-            stl' \<leftarrow> Graph.subtract_path_algo stl p;
+            stl' \<leftarrow> Graph.subtractPathRefine stl p;
             assert (Contained_Graph stl' stl \<and> Graph.E stl \<subseteq> Graph.E stl' \<union> set p);
-            stl' \<leftarrow> cleaning_algo (set Q_ls) stl';
+            stl' \<leftarrow> cleaningRefine (set Q_ls) stl';
             let f' = NFlow.augment c f' (NPreflow.augmentingFlow c f' p);
             RETURN (f', stl', False, True)
           }})
       (f, stl, False, False);
     RETURN (f', changed)}"
 
-
-
-
-
-find_theorems Graph.pathVertices set
-find_theorems Graph.pathVertices_fwd set
-find_theorems Graph.pathVertices
-thm Graph.pathVertices_append
-
-(*
-lemma (in Graph) aux: "u \<notin> set (pathVertices s p) \<Longrightarrow> (u, v) \<notin> set p"
-  by (induction p arbitrary: s) auto(*TODO*)
-lemma (in Graph) aux2: "u \<notin> set (pathVertices s p) \<Longrightarrow> (v, u) \<notin> set p"
-  apply (induction p arbitrary: s)
-   apply simp
-  apply simp sledgehammer
-  apply (induction p arbitrary: s rule: rev_induct)
-   apply simp
-  apply (simp add: Graph.pathVertices_append) apply auto
-  by (induction p arbitrary: s) auto(*TODO*)*)
-
-
-
-lemma dinitz_phase_concrete_refine: "dinitz_phase_concrete \<le> \<Down> Id dinitz_phase_assert"
-  unfolding dinitz_phase_concrete_def dinitz_phase_assert_def
-  apply refine_rcg
-            apply refine_dref_type
+lemma dinitzPhaseRefine_refine:
+  notes [refine_dref_pattern] = RELATESI_in_spec
+  shows "dinitzPhaseRefine \<le> \<Down> Id dinitzPhaseAssert"
+  unfolding dinitzPhaseRefine_def dinitzPhaseAssert_def
+  apply (refine_rcg, refine_dref_type)
            apply clarsimp_all
-  using cf.build_st_layering_correct apply simp
+  using cf.buildDualLayering_correct apply simp
+  defer apply (simp add: innerPathVertices_correct[symmetric])
 proof -
   fix f' stl changed
-  assume "dinitz_phase_assert_invar (f', stl, False, changed)"
-  then interpret bstu: Bounded_ST_Shortest_Path_Union stl "cf_of f'" s t "cf.min_dist s t"
-    unfolding dinitz_phase_assert_invar_def by blast
-  show "Graph.greedy_st_path_finding stl s t \<le> (select p. Graph.isPath stl s p t)"
-    using bstu.greedy_st_path_finding_correct .
+  assume "dinitzPhaseAssertInvar (f', stl, False, changed)"
+  then interpret bstu: Bounded_Dual_Shortest_Path_Union stl "cf_of f'" s t "cf.min_dist s t"
+    unfolding dinitzPhaseAssertInvar_def by blast
+  show "Graph.greedyPathFinding stl s t \<le> (select p. Graph.isPath stl s p t)"
+    using bstu.greedyPathFinding_correct .
 next
   fix f' stl p
-  assume "ST_Shortest_Path_Union stl (cf_of f') s t"
-  then interpret stu: ST_Shortest_Path_Union stl "cf_of f'" s t .
+  assume "Dual_Shortest_Path_Union stl (cf_of f') s t"
+  then interpret stu: Dual_Shortest_Path_Union stl "cf_of f'" s t .
 
   assume "Graph.isPath stl s p t"
   then have SP: "Graph.isPath stl s p t" by blast
-  
-  show "inner_path_vertices_algo p \<le> RES {tl (butlast (Graph.pathVertices s p))}"
-    using inner_path_vertices_algo_correct by (simp add: RES_sng_eq_RETURN)
 
-  from SP show "Graph.subtract_path_algo stl p \<le> RES {Graph.subtract_path stl p}"
-    using stu.g'.isSPath_distinct stu.paths_are_simple stu.g'.subtract_path_algo_correct
+  from SP show "Graph.subtractPathRefine stl p \<le> RES {Graph.subtract_path stl p}"
+    using stu.g'.isSPath_distinct stu.paths_are_simple stu.g'.subtractPathRefine_correct
     by (metis RES_sng_eq_RETURN)
 
-  thm Finite_Bounded_Graph.cleaning_algo_correct
   fix stl'
   assume "Contained_Graph stl' stl" "Graph.E stl \<subseteq> Graph.E stl' \<union> set p"
-  show "cleaning_algo (set (Graph.pathVertices s p) - {s, t}) stl' \<le> RES {cleaning s t stl'}"
+  show "cleaningRefine (set (Graph.pathVertices s p) - {s, t}) stl' \<le> RES {cleaning s t stl'}"
   proof (unfold RES_sng_eq_RETURN, intro Finite_Bounded_Graph.cleaning_algo_correct)
     show "s \<notin> set (Graph.pathVertices s p) - {s, t}"
       "t \<notin> set (Graph.pathVertices s p) - {s, t}"
@@ -1446,37 +1307,22 @@ next
   qed
 qed
 
-lemma dinitz_phase_concrete_correct: "dinitz_phase_concrete \<le> SPEC (\<lambda>(f', changed). res_dist_increasing_flow f' \<and> changed = (f' \<noteq> f) \<and> (changed \<longrightarrow> cf.connected s t))"
-  using dinitz_phase_concrete_refine dinitz_phase_assert_correct by simp
+lemma dinitzPhaseRefine_correct: "dinitzPhaseRefine \<le> SPEC (\<lambda>(f', changed). res_dist_increasing_flow f' \<and> changed = (f' \<noteq> f) \<and> (changed \<longrightarrow> cf.connected s t))"
+  using dinitzPhaseRefine_refine dinitzPhaseAssert_correct by simp
 end
+\<comment> \<open>Refining the assertion version\<close>
 
+subsection \<open>Dinitz outer loop refinement\<close>
 context Network
 begin
 (* TODO rework using changed flag *)
-definition dinitz_concrete :: "_ flow nres" where
-  "dinitz_concrete \<equiv> do {
-    (f, _) \<leftarrow> WHILE\<^sub>T snd (NFlow.dinitz_phase_concrete c s t \<circ> fst) (\<lambda>_. 0, True);
+definition dinitzRefine :: "_ flow nres" where
+  "dinitzRefine \<equiv> do {
+    (f, _) \<leftarrow> WHILE\<^sub>T snd (NFlow.dinitzPhaseRefine c s t \<circ> fst) (\<lambda>_. 0, True);
     RETURN f}"
 
-(*
-definition dinitz_concrete_aux_rel where
-  "dinitz_concrete_aux_rel \<equiv> {((f, m), f)|f m. m \<or> isMaxFlow f}"
-term dinitz_concrete_aux_rel
-thm dinitz_concrete_aux_rel_def
-
-thm bind_refine
-lemma dinitz_concrete_refine: "dinitz_concrete \<le> \<Down> Id dinitz"
-  unfolding dinitz_concrete_def dinitz_def
-  apply (refine_rcg bind_refine[where R'=dinitz_concrete_aux_rel])
-  unfolding dinitz_concrete_aux_rel_def apply clarsimp_all
-  defer using NFlow.dinitz_phase_concrete_refine apply clarsimp
-*)
-find_consts "('a \<Rightarrow> bool) \<Rightarrow> ('b \<Rightarrow> bool) \<Rightarrow> 'a \<times> 'b \<Rightarrow> bool"
-term pred_prod
-
-
-theorem dinitz_concrete_correct: "dinitz_concrete \<le> SPEC (\<lambda>f. isMaxFlow f)"
-  unfolding dinitz_concrete_def
+theorem dinitzRefine_correct: "dinitzRefine \<le> SPEC (\<lambda>f. isMaxFlow f)"
+  unfolding dinitzRefine_def
   apply (refine_vcg WHILET_rule[where I="\<lambda>(f', m). NFlow c s t f' \<and> (m \<or> isMaxFlow f')"
           and R="inv_image (less_than_bool <*lex*> res_dist_rel) prod.swap"])
       apply (fastforce simp: res_dist_wf)
@@ -1485,8 +1331,8 @@ proof -
   fix f
   assume "NFlow c s t f"
   then interpret NFlow c s t f .
-  have "dinitz_phase_concrete \<le> SPEC (\<lambda>(f', changed). res_dist_increasing_flow f' \<and> changed = (f' \<noteq> f) \<and> (changed \<longrightarrow> cf.connected s t))"
-    using dinitz_phase_concrete_correct .
+  have "dinitzPhaseRefine \<le> SPEC (\<lambda>(f', changed). res_dist_increasing_flow f' \<and> changed = (f' \<noteq> f) \<and> (changed \<longrightarrow> cf.connected s t))"
+    using dinitzPhaseRefine_correct .
   also have "... \<le> (spec s'. (case s' of (f', m) \<Rightarrow> NFlow c s t f' \<and> (m \<or> isMaxFlow f')) \<and> (prod.swap s', True, f) \<in> less_than_bool <*lex*> res_dist_rel)"
   proof (clarsimp, intro conjI)
     fix f'
@@ -1500,130 +1346,8 @@ proof -
     from CON_IF_NEQ show "f' = f \<longrightarrow> isMaxFlow f"
       using Graph.connected_def Graph.isSimplePath_fwd n'.fofu_III_I n'.fofu_II_III n'.isAugmentingPath_def DIST by blast
   qed 
-  finally show "dinitz_phase_concrete \<le> (spec s'. (case s' of (f', m) \<Rightarrow> NFlow c s t f' \<and> (m \<or> isMaxFlow f')) \<and> (prod.swap s', True, f) \<in> less_than_bool <*lex*> res_dist_rel)" .
+  finally show "dinitzPhaseRefine \<le> (spec s'. (case s' of (f', m) \<Rightarrow> NFlow c s t f' \<and> (m \<or> isMaxFlow f')) \<and> (prod.swap s', True, f) \<in> less_than_bool <*lex*> res_dist_rel)" .
 qed
-
-(*
-term SPEC
-term "if changed then cf.connected s t \<and> res_dist_increasing_flow f' else \<not> cf.connected s t \<and> (f' = f))"
-lemma (in NFlow) dinitz_phase_concrete_correct_if:
-  "dinitz_phase_concrete \<le> SPEC (\<lambda>(f', changed).
-    (if changed then cf.connected s t \<and> res_dist_increasing_flow f' else \<not> cf.connected s t \<and> (f' = f)))"
-
-
-res_dist_increasing_flow f' \<and> changed = (cf.connected s t \<and> f' \<noteq> f))"
-  sorry*)
-
-
-
-(*
-term "inv_image (less_than_bool <*lex*> res_dist_rel) prod.swap"
-theorem dinitz_concrete_correct: "dinitz_concrete \<le> SPEC (\<lambda>f. isMaxFlow f)"
-  unfolding dinitz_concrete_def
-  apply (refine_vcg WHILET_rule[where I="\<lambda>(f', m). NFlow c s t f' \<and> (m \<or> isMaxFlow f')"
-          and R="inv_image (less_than_bool <*lex*> res_dist_rel) prod.swap"])
-      apply (fastforce simp: res_dist_wf)
-     apply (simp add: NFlowI Network_axioms zero_is_flow)
-    apply simp
-   defer apply simp
-
-proof clarsimp
-  fix f
-  assume "NFlow c s t f"
-  then interpret n: NFlow c s t f .
-  thm n.dinitz_phase_concrete_correct
-  have "n.dinitz_phase_concrete \<le> SPEC (\<lambda>(f', changed). n.res_dist_increasing_flow f' \<and> changed = (f' \<noteq> f))"
-    using n.dinitz_phase_concrete_correct .
-  also have "... \<le> (spec s'. (case s' of (f', m) \<Rightarrow> NFlow c s t f' \<and> (m \<or> isMaxFlow f')) \<and> (prod.swap s', True, f) \<in> less_than_bool <*lex*> res_dist_rel)"
-  proof (clarsimp, intro conjI)
-    fix f'
-    assume "n.res_dist_increasing_flow f'"
-    then show "NFlow c s t f'"
-      unfolding n.res_dist_increasing_flow_def by simp
-    then interpret n': NFlow c s t f' .
-    from \<open>n.res_dist_increasing_flow f'\<close> have DIST: "n'.cf.connected s t \<longrightarrow> n.cf.min_dist s t < n'.cf.min_dist s t"
-      unfolding n.res_dist_increasing_flow_def by simp
-
-    then show "NFlow c s t f' \<and> (f' = f \<longrightarrow> isMaxFlow f) \<and> (f' = f \<or> f' \<noteq> f \<and> (f', f) \<in> res_dist_rel)"
-      unfolding n.res_dist_increasing_flow_def apply auto
-        apply (meson Graph.connected_def Graph.isSimplePath_fwd n.ford_fulkerson(1) n.isAugmentingPath_def)
-      unfolding res_dist_rel_def apply auto oops
-
-
-      thm res_dist_rel_def
-
-theorem dinitz_concrete_correct: "dinitz_concrete \<le> SPEC (\<lambda>f. isMaxFlow f)"
-  unfolding dinitz_concrete_def
-  apply (refine_vcg WHILET_rule[where I="\<lambda>(f', m). NFlow c s t f' \<and> (m \<or> isMaxFlow f')"
-          and R="inv_image (less_than_bool <*lex*> res_dist_rel) prod.swap"])
-      apply (fastforce simp: res_dist_wf)
-     apply (simp add: NFlowI Network_axioms zero_is_flow)
-    apply simp
-   defer apply simp
-
-proof clarsimp
-  fix f
-  assume "NFlow c s t f"
-  then interpret n: NFlow c s t f .
-  thm n.dinitz_phase_concrete_correct'
-  have "n.dinitz_phase_concrete \<le> SPEC (\<lambda>(f', changed). n.res_dist_increasing_flow f' \<and> (changed \<longleftrightarrow> n.val < Flow.val c s f'))"
-    using n.dinitz_phase_concrete_correct' sorry
-  also have "... \<le> (spec s'. (case s' of (f', m) \<Rightarrow> NFlow c s t f' \<and> (m \<or> isMaxFlow f')) \<and> (prod.swap s', True, f) \<in> less_than_bool <*lex*> res_dist_rel)"
-  proof (clarsimp, intro conjI)
-    fix f'
-    assume "n.res_dist_increasing_flow f'"
-    then show "NFlow c s t f'"
-      unfolding n.res_dist_increasing_flow_def by simp
-    then interpret n': NFlow c s t f' .
-
-    from \<open>n.res_dist_increasing_flow f'\<close> have DIST: "n'.cf.connected s t \<longrightarrow> n.cf.min_dist s t < n'.cf.min_dist s t"
-      unfolding n.res_dist_increasing_flow_def by simp
-    then show "n.val < n'.val \<or> isMaxFlow f'" apply auto
-       apply (simp add: n'.ford_fulkerson(1) Graph.connected_def Graph.isSimplePath_fwd n'.isAugmentingPath_def)
-      sorry
-
-    from DIST show "n.val < n'.val \<longrightarrow> (f', f) \<in> res_dist_rel"
-      unfolding res_dist_rel_def
-      apply auto
-      by (meson Graph.connected_def Graph.isSimplePath_fwd isMaxFlow_def less_le_not_le n'.Flow_axioms n.fofu_III_I n.fofu_II_III n.isAugmentingPath_def)+
-
-    oops
-
-theorem dinitz_concrete_correct: "dinitz_concrete \<le> SPEC (\<lambda>f. isMaxFlow f)"
-  unfolding dinitz_concrete_def
-  apply (refine_vcg WHILET_rule[where I="\<lambda>(f', m). NFlow c s t f' \<and> (m \<or> isMaxFlow f')"
-          and R="inv_image (less_than_bool <*lex*> res_dist_rel) prod.swap"])
-      apply (fastforce simp: res_dist_wf)
-     apply (simp add: NFlowI Network_axioms zero_is_flow)
-    apply simp
-   defer apply simp
-
-proof clarsimp
-  fix f
-  assume "NFlow c s t f"
-  then interpret n: NFlow c s t f .
-  thm n.dinitz_phase_concrete_correct'
-  have "n.dinitz_phase_concrete \<le> SPEC (\<lambda>(f', changed). n.res_dist_increasing_flow f' \<and> (changed \<or> f' = f \<and> isMaxFlow f))"
-    using n.dinitz_phase_concrete_correct' .
-  also have "... \<le> (spec s'. (case s' of (f', m) \<Rightarrow> NFlow c s t f' \<and> (m \<or> isMaxFlow f')) \<and> (prod.swap s', True, f) \<in> less_than_bool <*lex*> res_dist_rel)"
-  proof (clarsimp, intro conjI)
-    fix f'
-    assume "n.res_dist_increasing_flow f'"
-    then show "NFlow c s t f'"
-      unfolding n.res_dist_increasing_flow_def by simp
-    then interpret n': NFlow c s t f' .
-
-    from \<open>n.res_dist_increasing_flow f'\<close> have DIST: "n'.cf.connected s t \<longrightarrow> n.cf.min_dist s t < n'.cf.min_dist s t"
-      unfolding n.res_dist_increasing_flow_def by simp
-    then show "n.val < n'.val \<or> isMaxFlow f'" apply auto
-       apply (simp add: n'.ford_fulkerson(1) Graph.connected_def Graph.isSimplePath_fwd n'.isAugmentingPath_def)
-      sorry
-
-    from DIST show "n.val < n'.val \<longrightarrow> (f', f) \<in> res_dist_rel"
-      unfolding res_dist_rel_def
-      apply auto
-      by (meson Graph.connected_def Graph.isSimplePath_fwd isMaxFlow_def less_le_not_le n'.Flow_axioms n.fofu_III_I n.fofu_II_III n.isAugmentingPath_def)+
-
-      oops*)
 end
+\<comment> \<open>Dinitz outer loop refinement\<close>
 end
